concurrency/compcert_threads.v
@@ -2,7 +2,7 @@ Require Import Axioms.
 
 Add LoadPath "../sepcomp" as sepcomp.
 
-(* Require Import sepcomp. Import SepComp. *)
+Require Import sepcomp. Import SepComp.
 Require Import semantics_lemmas.
 
 
